theories/Dot/operational.v
@@ -84,12 +84,21 @@ Qed.
 
 End saved_interp.
 
+Implicit Types
+         (T: ty) (v: vl) (t e: tm) (d: dm) (ds: dms) (vs: vls)
+         (Γ : ctx).
 (** Substitute object inside itself (to give semantics to the "self"
     variable). To use when descending under the [vobj] binder. *)
-Definition selfSubst (ds: dms): dms := ds.|[vobj ds/].
+Definition selfSubst ds: dms := ds.|[vobj ds/].
 
-Definition objLookup v l d: Prop :=
-  ∃ ds, v = vobj ds ∧ reverse (selfSubst ds) !! l = Some d.
+(* Unset Program Cases. *)
+(* Definition gmap_of_dms ds: gmap label dm := map_of_list ds. *)
+(* Definition dms_lookup l ds := gmap_of_dms ds !! l. *)
+(* Arguments gmap_of_dms /. *)
+(* Arguments dms_lookup /. *)
+
+Definition objLookup v (l: label) d: Prop :=
+  ∃ ds, v = vobj ds ∧ (dms_lookup l (selfSubst ds)) = Some d.
 Notation "v @ l ↘ d" := (objLookup v l d) (at level 20).
 
 (** Instead of letting obj_opens_to autounfold,
@@ -113,98 +122,116 @@ Ltac objLookupDet :=
     assert (d2 = d1) as ? by (eapply objLookupDet; eassumption); injectHyps
   end.
 
-Section AboutObjLookup.
+(* Section AboutObjLookup. *)
 (** Auxiliary definitions to prove [lookup_reverse_length], since a direct inductive proof appers to fail (but
 see rev_append_map for an approach that has a chance). *)
-Fixpoint indexr {X} (i: nat) (xs: list X) : option X :=
-  match xs with
-  | [] => None
-  | x :: xs =>
-    if decide (i = length xs) then Some x else indexr i xs
-  end.
+(* Fixpoint indexr {X} (i: nat) (xs: list X) : option X := *)
+(*   match xs with *)
+(*   | [] => None *)
+(*   | x :: xs => *)
+(*     if decide (i = length xs) then Some x else indexr i xs *)
+(*   end. *)
 
-Lemma indexr_max {X} (T: X) i vs:
-                       indexr i vs = Some T ->
-                       i < length vs.
-Proof.
-  induction vs; first done; rewrite /lt in IHvs |- *; move => /= H.
-  case_decide; subst; [ lia | eauto ].
-Qed.
-Hint Resolve indexr_max.
-
-Lemma lookup_reverse_indexr {X} (ds: list X) l: reverse ds !! l = indexr l ds.
-Proof.
-  elim: ds l => [|d ds IHds] l //=.
-  case_decide; subst.
-  - by rewrite reverse_cons lookup_app_r reverse_length ?Nat.sub_diag.
-  - case (decide (l < length ds)) => Hl.
-    + by rewrite reverse_cons lookup_app_l ?reverse_length.
-    + assert (l > length ds) by omega.
-      assert (indexr l ds = None). {
-        destruct (indexr l ds) eqn:? => //.
-        assert (l < length ds) by (eapply indexr_max; eauto).
-        lia.
-      }
-      by rewrite lookup_ge_None_2 ?reverse_length.
-Qed.
-
-Lemma lookup_reverse_length {X} l (d: X) ds: l = length ds → reverse (d :: ds) !! l = Some d.
-Proof.
-  intros; subst. rewrite lookup_reverse_indexr /=. case_decide => //=.
-Qed.
-
-Lemma obj_lookup_cons d ds: vobj (d :: ds) @ length ds ↘ d.|[vobj (d :: ds)/].
-Proof.
-  hnf. eexists; split; trivial.
-  rewrite /selfSubst /=. apply lookup_reverse_length. by rewrite map_length.
-Qed.
-
-Lemma indexr_extend {X} vs n x (T: X):
-                       indexr n vs = Some T ->
-                       indexr n (x::vs) = Some T.
-Proof.
-  move => H /=; assert (n < length vs) by naive_solver; by case_decide; first lia.
-Qed.
-Hint Resolve indexr_extend.
-
-Lemma lookup_reverse_extend {X} l (d: X) ds:
-  reverse ds !! l = Some d →
-  reverse (d :: ds) !! l = Some d.
-Proof.
-  intros; subst. rewrite -> lookup_reverse_indexr in *. by apply indexr_extend.
-Qed.
-
-Lemma rev_append_map {X Y} (xs1 xs2: list X) (f: X → Y): rev_append (map f xs1) (map f xs2) = map f (rev_append xs1 xs2).
-Proof.
-  elim: xs1 xs2 => [|x xs1 IH] xs2 //=. eapply (IH (x :: xs2)).
-Qed.
-Lemma reverse_map {X Y} (xs: list X) (f: X → Y): reverse (map f xs) = map f (reverse xs).
-Proof. rewrite /reverse. eapply (rev_append_map xs []). Qed.
-
-Lemma lookup_map {X Y} x (xs: list X) (f: X → Y) l: xs !! l = Some x → map f xs !! l = Some (f x).
-Proof.
-  elim: xs l => /= [|x' xs IH] [|l] //= Hl; by [cinject Hl | apply IH].
-Qed.
-
-(* Lemma lookup_map_inv {X Y} x (xs: list X) (f: X → Y) l: map f xs !! l = Some (f x) → xs !! l = Some x. *)
+(* Lemma indexr_max {X} (x: X) i xs: *)
+(*                        indexr i xs = Some x -> *)
+(*                        i < length xs. *)
 (* Proof. *)
-(*   elim: xs l => [|x' xs IH] [|l] //=. (* ONLY FOR F INDUCTIVE! *) *)
+(*   induction xs; first done; rewrite /lt in IHxs |- *; move => /= H. *)
+(*   case_decide; subst; [ lia | eauto ]. *)
+(* Qed. *)
+(* Hint Resolve indexr_max. *)
 
-(* Lemma obj_lookup_extend d ds l: *)
-(*   vobj ds @ l ↘ d.|[vobj ds/] → *)
-(*   vobj (d :: ds) @ l ↘ d.|[vobj (d :: ds)/]. *)
+(* Lemma lookup_reverse_indexr {X} (ds: list X) l: reverse ds !! l = indexr l ds. *)
 (* Proof. *)
-(*   hnf. *)
-(*   intros (ds0 & Heq & Hl). cinject Heq. *)
-(*   eexists; split; trivial. *)
-(*   move: Hl. rewrite /selfSubst /lookup_reverse_indexr /= => Hl. *)
-(*   apply lookup_reverse_extend. *)
-(*   move: Hl. rewrite /hsubst /HSubst_dm !reverse_map => Hl. *)
-(*   apply lookup_map. apply lookup_map_inv in Hl. apply Hl. *)
-(*   (* eauto using lookup_map, lookup_map_inv. *) *)
+(*   elim: ds l => [|d ds IHds] l //=. *)
+(*   case_decide; subst. *)
+(*   - by rewrite reverse_cons lookup_app_r reverse_length ?Nat.sub_diag. *)
+(*   - case (decide (l < length ds)) => Hl. *)
+(*     + by rewrite reverse_cons lookup_app_l ?reverse_length. *)
+(*     + assert (l > length ds) by omega. *)
+(*       assert (indexr l ds = None). { *)
+(*         destruct (indexr l ds) eqn:? => //. *)
+(*         assert (l < length ds) by (eapply indexr_max; eauto). *)
+(*         lia. *)
+(*       } *)
+(*       by rewrite lookup_ge_None_2 ?reverse_length. *)
 (* Qed. *)
 
-End AboutObjLookup.
+(* Lemma lookup_reverse_length {X} l (x: X) xs: l = length xs → reverse (x :: xs) !! l = Some x. *)
+(* Proof. *)
+(*   intros; subst. rewrite lookup_reverse_indexr /=. case_decide => //=. *)
+(* Qed. *)
+
+(* Lemma obj_lookup_cons d ds l: (l, d) ∈ ds → vobj ds @ l ↘ d.|[vobj ds/]. *)
+(* Proof. *)
+(*   hnf; move => Hin; eexists; split => //=. *)
+(*   elim: ds Hin => [|[l' d'] ds IHds] //= Hin; first inversion Hin. *)
+(*   (* destruct (decide (l = l')) as [-> | Hne]. *) *)
+(*   inverse Hin; rewrite ?lookup_insert /mapsnd //=. *)
+(*   apply IHds in H1. *)
+(*   destruct (decide (l = l')) as [Heq | Hne]. *)
+(*   admit. *)
+(*   cbn. *)
+(*   asimpl. cbn. *)
+(*   f_equal. *)
+(*   rewrite /selfSubst /=. *)
+  
+(*   assert ((l, d.|[vobj ds/]) ∈ ds.|[vobj ds/]). *)
+(*   rewrite /hsubst /list_pair_hsubst -/mapsnd. *)
+(*   set (sb := (hsubst (vobj ds .: ids))). *)
+(*   assert (map (mapsnd ) (l, d.|[vobj ds/]) ∈ ds.|[vobj ds/]). *)
+  
+(*   Search "_ ∈ _". *)
+(*   assert ((l, d) ∈ gmap_of_dms ds). *)
+(*   apply lookup_reverse_length. by rewrite map_length. *)
+(* Qed. *)
+
+(* Lemma indexr_extend {X} vs n x (T: X): *)
+(*                        indexr n vs = Some T -> *)
+(*                        indexr n (x::vs) = Some T. *)
+(* Proof. *)
+(*   move => H /=; assert (n < length vs) by naive_solver; by case_decide; first lia. *)
+(* Qed. *)
+(* Hint Resolve indexr_extend. *)
+
+(* Lemma lookup_reverse_extend {X} l (d: X) ds: *)
+(*   reverse ds !! l = Some d → *)
+(*   reverse (d :: ds) !! l = Some d. *)
+(* Proof. *)
+(*   intros; subst. rewrite -> lookup_reverse_indexr in *. by apply indexr_extend. *)
+(* Qed. *)
+
+(* Lemma rev_append_map {X Y} (xs1 xs2: list X) (f: X → Y): rev_append (map f xs1) (map f xs2) = map f (rev_append xs1 xs2). *)
+(* Proof. *)
+(*   elim: xs1 xs2 => [|x xs1 IH] xs2 //=. eapply (IH (x :: xs2)). *)
+(* Qed. *)
+(* Lemma reverse_map {X Y} (xs: list X) (f: X → Y): reverse (map f xs) = map f (reverse xs). *)
+(* Proof. rewrite /reverse. eapply (rev_append_map xs []). Qed. *)
+
+(* Lemma lookup_map {X Y} x (xs: list X) (f: X → Y) l: xs !! l = Some x → map f xs !! l = Some (f x). *)
+(* Proof. *)
+(*   elim: xs l => /= [|x' xs IH] [|l] //= Hl; by [cinject Hl | apply IH]. *)
+(* Qed. *)
+
+(* (* Lemma lookup_map_inv {X Y} x (xs: list X) (f: X → Y) l: map f xs !! l = Some (f x) → xs !! l = Some x. *) *)
+(* (* Proof. *) *)
+(* (*   elim: xs l => [|x' xs IH] [|l] //=. (* ONLY FOR F INDUCTIVE! *) *) *)
+
+(* (* Lemma obj_lookup_extend d ds l: *) *)
+(* (*   vobj ds @ l ↘ d.|[vobj ds/] → *) *)
+(* (*   vobj (d :: ds) @ l ↘ d.|[vobj (d :: ds)/]. *) *)
+(* (* Proof. *) *)
+(* (*   hnf. *) *)
+(* (*   intros (ds0 & Heq & Hl). cinject Heq. *) *)
+(* (*   eexists; split; trivial. *) *)
+(* (*   move: Hl. rewrite /selfSubst /lookup_reverse_indexr /= => Hl. *) *)
+(* (*   apply lookup_reverse_extend. *) *)
+(* (*   move: Hl. rewrite /hsubst /HSubst_dm !reverse_map => Hl. *) *)
+(* (*   apply lookup_map. apply lookup_map_inv in Hl. apply Hl. *) *)
+(* (*   (* eauto using lookup_map, lookup_map_inv. *) *) *)
+(* (* Qed. *) *)
+
+(* End AboutObjLookup. *)
 
 (** Instantiating iris with  *)
 Module lang.
@@ -236,7 +263,7 @@ Inductive head_step : tm -> state -> list observation -> tm -> state -> list tm 
 | st_beta t1 v2 σ:
     head_step (tapp (tv (vabs t1)) (tv v2)) σ [] (t1.|[v2/]) σ []
 | st_proj ds l σ v:
-    reverse (selfSubst ds) !! l = Some (dvl v) ->
+    dms_lookup l (selfSubst ds) = Some (dvl v) ->
     head_step (tproj (tv (vobj ds)) l) σ [] (tv v) σ []
 | st_skip t σ:
     head_step (tskip t) σ [] t σ [].
